try different instruction normalization

theories/automation.v
@@ -110,6 +110,9 @@ Proof. split; naive_solver. Qed.
 Global Instance simpl_SReadMem a1 a2 v1 v2:
   SimplBoth (SReadMem a1 v1 = SReadMem a2 v2) (a1 = a2 ∧ v1 = v2).
 Proof. split; naive_solver. Qed.
+Global Instance simpl_SInstrTrap a1 a2:
+  SimplBoth (SInstrTrap a1 = SInstrTrap a2) (a1 = a2).
+Proof. split; naive_solver. Qed.
 
 Global Instance simpl_impl_valu_has_shape_bits v n:
   SimplImpl true (valu_has_shape v (BitsShape n)) (λ T, ∀ b : bv n, v = RVal_Bits b → T).
@@ -176,6 +179,28 @@ Proof.
       rewrite !Z.land_spec Z.lor_spec Z.shiftl_spec ?Z.bits_0 ?(Z.ones_spec_low 3); [|lia..].
       by simplify_bool_eq.
 Qed.
+
+(** * [normalize_instr_addr] *)
+
+Definition normalize_instr_addr (a1 a2 : Z) : Prop := bv_wrap 64 a1 = bv_wrap 64 a2.
+Typeclasses Opaque normalize_instr_addr.
+
+Class NormalizeInstrAddr (a1 a2 : Z) : Prop :=
+  normalize_instr_addr_proof : normalize_instr_addr a1 a2.
+
+Global Instance simpl_and_normalize_instr_addr a1 a2 a2' `{!NormalizeInstrAddr a1 a2'} `{!IsProtected a2} :
+  SimplAndUnsafe true (normalize_instr_addr a1 a2) (λ T, a2' = a2 ∧ T).
+Proof. unfold NormalizeInstrAddr, SimplAndUnsafe in *. naive_solver. Qed.
+
+Ltac solve_normalize_instr_addr :=
+  unfold NormalizeInstrAddr, normalize_instr_addr; unLET;
+  try lazymatch goal with
+  | |- bv_wrap _ ?a = _ => reduce_closed a
+  end;
+  exact: eq_refl.
+
+Global Hint Extern 10 (NormalizeInstrAddr _ _) =>
+  solve_normalize_instr_addr : typeclass_instances.
 
 (** * Registering extensions *)
 (** More automation for modular arithmetics. *)
@@ -762,11 +787,11 @@ Section instances.
     λ T, i2p (simpl_goal_reg_col_cons r col s T).
 
   Lemma li_wp_next_instr:
-    (∃ (nPC newPC : addr),
+    (∃ (nPC newPC : addr) normPC,
      arch_pc_reg ↦ᵣ RVal_Bits nPC ∗
-     vm_compute_hint (λ b, Some (bv_unsigned b)) nPC (λ a,
-     ⌜Z_to_bv_checked 64 a = Some newPC⌝ ∗
-     find_in_context (FindInstrKind a true) (λ ik,
+     ⌜normalize_instr_addr (bv_unsigned nPC) normPC⌝ ∗
+     ⌜newPC = Z_to_bv 64 normPC⌝ ∗
+     find_in_context (FindInstrKind normPC true) (λ ik,
      match ik with
      | IKInstr (Some ts) =>
        ⌜ts ≠ []⌝ ∗ [∧ list] t∈ts, arch_pc_reg ↦ᵣ RVal_Bits newPC -∗ WPasm t
@@ -774,9 +799,11 @@ Section instances.
        ∃ Pκs, spec_trace Pκs ∗ ⌜scons (SInstrTrap newPC) snil ⊆ Pκs⌝ ∗ True
      | IKPre l P => P
      end
-    ))) -∗
+    )) -∗
     WPasm [].
   Proof.
+  Admitted.
+  (*
     iDestruct 1 as (??) "(HPC&%a&%Ha&%Hchecked&Hwp)". case: Ha => ?. subst.
     rewrite ->Z_to_bv_checked_bv_unsigned in *; simplify_eq.
     iDestruct "Hwp" as (ins) "[Hi Hwp]".
@@ -791,10 +818,12 @@ Section instances.
       spec_solver.
     - by iApply (wp_next_instr_pre with "[$] [$]").
   Qed.
-
+*)
   Lemma li_instr_pre l a P:
-    (∃ newPC, ⌜Z_to_bv_checked 64 a = Some newPC⌝ ∗
-     find_in_context (FindInstrKind a l) (λ ik,
+    (∃ newPC normPC,
+     ⌜normalize_instr_addr a normPC⌝ ∗
+     ⌜newPC = Z_to_bv 64 normPC⌝ ∗
+     find_in_context (FindInstrKind normPC l) (λ ik,
      match ik with
      | IKInstr (Some ts) =>
        ⌜ts ≠ []⌝ ∗ [∧ list] t∈ts, P -∗ arch_pc_reg ↦ᵣ RVal_Bits newPC -∗ WPasm t
@@ -804,7 +833,9 @@ Section instances.
      end
     )) -∗
     instr_pre' l a P.
-  Proof.
+  Proof. Admitted.
+  (*
+
     iDestruct 1 as (?->%Z_to_bv_checked_Some ins) "[Hinstr Hwp]".
     destruct ins as [[?|]|?] => /=.
     - iDestruct "Hwp" as (?) "Hl".
@@ -819,7 +850,7 @@ Section instances.
     - iDestruct "Hwp" as (?) "Hwand".
       by iApply (instr_pre_wand with "Hinstr").
   Qed.
-
+*)
   Lemma li_wp_read_reg r v ann es :
     (find_in_context (FindRegMapsTo r) (λ rk,
       match rk with
